botred.v
@@ -1,10 +1,13 @@
 
 Require Import beta.
+Require Import cases.
 
 Section Botred.
 
 Variable U : term -> Prop.
 Variable Hm : meaningless U.
+
+(************************************************************************************************)
 
 Lemma lem_par_bot_refl_0 : forall x, par_bot U x x.
 Proof.
@@ -15,6 +18,53 @@ Lemma lem_par_bot_refl : forall x y, x == y -> par_bot U x y.
 Proof.
   coinduction.
 Qed.
+
+Lemma lem_par_bot_preserves_U : forall t s, U t -> par_bot U t s -> U s.
+Proof.
+  pose lem_par_bot_to_sim; ycrush.
+Qed.
+
+Lemma lem_par_bot_preserves_U_rev : forall t s, U t -> par_bot U s t -> U s.
+Proof.
+  pose lem_par_bot_to_sim; pose lem_sim_sym; unfold symmetric in *; ycrush.
+Qed.
+
+Lemma lem_par_bot_preserves_bot_redex_rev :
+  forall x y z, par_bot U x y -> bot_redex U y z -> bot_redex U x z.
+Proof.
+  unfold bot_redex; pose lem_par_bot_preserves_U_rev; ycrush.
+Qed.
+
+Lemma lem_par_bot_trans : transitive term (par_bot U).
+Proof.
+  coinduction CH on 4 using auto.
+  - clear CH; pose lem_par_bot_preserves_bot_redex_rev; ycrush.
+  - revert H; csolve CH using eauto.
+    unfold bot_redex in *; clear CH; ycrush.
+  - revert H; csolve CH using eauto.
+    unfold bot_redex in *; clear CH; ycrush.
+Qed.
+
+Lemma lem_step_bot_to_par_bot : forall t s, step_bot U t s -> par_bot U t s.
+Proof.
+  pose lem_par_bot_refl; coinduction.
+Qed.
+
+Lemma lem_par_bot_app :
+  forall t s1 s2, par_bot U t (app s1 s2) ->
+                  exists t1 t2, t = app t1 t2 /\ par_bot U t1 s1 /\ par_bot U t2 s2.
+Proof.
+  destruct t; intros ? ? H; inversion H; subst; ycrush.
+Qed.
+
+Lemma lem_par_bot_abs :
+  forall t s, par_bot U t (abs s) ->
+                  exists u, t = abs u /\ par_bot U u s.
+Proof.
+  destruct t; intros ? H; inversion H; subst; ycrush.
+Qed.
+
+(************************************************************************************************)
 
 Lemma lem_U_morphism : forall x y, U x -> x == y -> U y.
 Proof.
@@ -32,7 +82,7 @@ Qed.
 Lemma lem_par_bot_morphism : morphism (par_bot U).
 Proof.
   unfold morphism.
-  coinduction CH using auto.
+  coinduct CH.
   - clear CH; pose lem_bot_redex_morphism; ycrush.
   - revert H; csolve CH.
   - revert H; csolve CH.
@@ -43,8 +93,10 @@ Proof.
     constructor 4.
     + apply CH with (x := x0) (y := x'); pose_term_eq; eauto.
     + pose_term_eq; ycrush.
-  - clear H0; revert H; csolve CH.
-    clear CH; sauto.
+  - clear H0; revert H; cintro.
+    + clear CH; sauto.
+    + destruct x', y'; try solve [ clear CH; sauto ].
+      pose_term_eq; cosolve CH.
 Qed.
 
 Add Parametric Morphism : (bot_redex U) with
@@ -108,8 +160,527 @@ Proof.
   - clear CH; intros; autorewrite with shints; repeat ysplit; try bomega.
     + eauto using lem_par_bot_refl_0.
     + eauto using lem_par_bot_shift_closed.
-  - revert H; csolve CH.
-  - revert H; csolve CH.
+Qed.
+
+(************************************************************************************************)
+
+Lemma lem_beta_bot_redex_morphism : morphism (beta_bot_redex U).
+Proof.
+  unfold morphism, beta_bot_redex.
+  pose lem_beta_redex_morphism; pose lem_bot_redex_morphism; ycrush.
+Qed.
+
+Lemma lem_step_beta_bot_morphism : morphism (step_beta_bot U).
+Proof.
+  unfold step_beta_bot.
+  apply lem_comp_morphism.
+  apply lem_beta_bot_redex_morphism.
+Qed.
+
+Lemma lem_red_beta_bot_morphism : morphism (red_beta_bot U).
+Proof.
+  unfold red_beta.
+  apply lem_star_morphism.
+  apply lem_step_beta_bot_morphism.
+Qed.
+
+Lemma lem_inf_beta_bot_morphism : morphism (inf_beta_bot U).
+Proof.
+  unfold inf_beta.
+  apply lem_inf_morphism.
+  apply lem_step_beta_bot_morphism.
+Qed.
+
+Add Parametric Morphism : (beta_bot_redex U) with
+    signature term_eq ==> term_eq ==> iff as beta_bot_redex_mor.
+Proof.
+  split; intro; eapply lem_beta_bot_redex_morphism; pose_term_eq; eauto.
+Qed.
+
+Add Parametric Morphism : (step_beta_bot U) with
+    signature term_eq ==> term_eq ==> iff as step_beta_bot_mor.
+Proof.
+  split; intro; eapply lem_step_beta_bot_morphism; pose_term_eq; eauto.
+Qed.
+
+Add Parametric Morphism : (red_beta_bot U) with
+    signature term_eq ==> term_eq ==> iff as red_beta_bot_mor.
+Proof.
+  split; intro; eapply lem_red_beta_bot_morphism; pose_term_eq; eauto.
+Qed.
+
+Add Parametric Morphism : (inf_beta_bot U) with
+    signature term_eq ==> term_eq ==> iff as inf_beta_bot_mor.
+Proof.
+  split; intro; eapply lem_inf_beta_bot_morphism; pose_term_eq; eauto.
+Qed.
+
+(************************************************************************************************)
+
+Lemma lem_step_beta_bot_redex_beta : forall x y, step_beta_bot U (app (abs x) y) (x [0 := y]).
+Proof.
+  constructor; constructor; econstructor; pose_term_eq; eauto.
+Qed.
+
+Lemma lem_step_beta_bot_redex_bot : forall x, U x -> x != bot -> step_beta_bot U x bot.
+Proof.
+  constructor; constructor 2; econstructor; pose_term_eq; eauto.
+Qed.
+
+Lemma lem_red_beta_bot_refl : forall x y, x == y -> red_beta_bot U x y.
+Proof.
+  apply lem_red_refl; apply lem_beta_bot_redex_morphism.
+Qed.
+
+Lemma lem_red_beta_bot_refl_0 : reflexive term (red_beta_bot U).
+Proof.
+  apply lem_red_refl_0; apply lem_beta_bot_redex_morphism.
+Qed.
+
+Lemma lem_red_beta_bot_trans : transitive term (red_beta_bot U).
+Proof.
+  apply lem_red_trans; apply lem_beta_bot_redex_morphism.
+Qed.
+
+Lemma lem_red_beta_bot_step : forall x y z, step_beta_bot U x y -> red_beta_bot U y z -> red_beta_bot U x z.
+Proof.
+  apply lem_red_step; apply lem_beta_bot_redex_morphism.
+Qed.
+
+Lemma lem_red_beta_bot_app : forall x x' y y', red_beta_bot U x x' -> red_beta_bot U y y' ->
+                                               red_beta_bot U (app x y) (app x' y').
+Proof.
+  apply lem_red_app; apply lem_beta_bot_redex_morphism.
+Qed.
+
+Lemma lem_red_beta_bot_abs : forall x x', red_beta_bot U x x' -> red_beta_bot U (abs x) (abs x').
+Proof.
+  apply lem_red_abs; apply lem_beta_bot_redex_morphism.
+Qed.
+
+Lemma lem_red_beta_bot_step_rev : forall x y z, red_beta_bot U x y -> step_beta_bot U y z -> red_beta_bot U x z.
+Proof.
+  apply lem_red_step_rev; apply lem_beta_bot_redex_morphism.
+Qed.
+
+Lemma lem_red_beta_bot_redex_beta : forall x y, red_beta_bot U (app (abs x) y) (x [0 := y]).
+Proof.
+  intros; econstructor; econstructor 2.
+  - eauto using lem_step_beta_bot_redex_beta.
+  - constructor; pose_term_eq; eauto.
+Qed.
+
+Lemma lem_red_beta_bot_redex_bot : forall x y, bot_redex U x y -> red_beta_bot U x y.
+Proof.
+  unfold bot_redex.
+  intros; simp_hyps; econstructor; econstructor 2.
+  - eauto using lem_step_beta_bot_redex_bot.
+  - constructor; pose_term_eq; eauto.
+Qed.
+
+Lemma lem_red_beta_bot_redex_U : forall t, U t -> red_beta_bot U t bot.
+Proof.
+  intros t H.
+  assert (HH: bot_redex U t bot \/ t = bot) by
+      (unfold bot_redex; destruct t; eauto; left; ycrush).
+  destruct HH.
+  - apply lem_red_beta_bot_redex_bot; assumption.
+  - apply lem_red_beta_bot_refl; ycrush.
+Qed.
+
+Lemma lem_step_beta_bot_to_red_beta_bot : forall x y, step_beta_bot U x y -> red_beta_bot U x y.
+Proof.
+  apply lem_step_to_red; apply lem_beta_bot_redex_morphism.
+Qed.
+
+Lemma lem_step_beta_to_step_beta_bot : forall x y, step_beta x y -> step_beta_bot U x y.
+Proof.
+  induction 1; ycrush.
+Qed.
+
+Lemma lem_step_beta_to_red_beta_bot : forall x y, step_beta x y -> red_beta_bot U x y.
+Proof.
+  pose lem_step_beta_to_step_beta_bot; pose lem_step_to_red; pose lem_beta_bot_redex_morphism.
+  unfold red_beta_bot, step_beta_bot, step_beta, red in *.
+  ycrush.
+Qed.
+
+Lemma lem_red_beta_to_red_beta_bot : forall x y, red_beta x y -> red_beta_bot U x y.
+Proof.
+  intros x y H.
+  destruct H as [n H].
+  induction H.
+  - ycrush.
+  - pose lem_step_beta_to_red_beta_bot; pose lem_red_beta_bot_trans; ycrush.
+Qed.
+
+Ltac pose_red_beta_bot :=
+  pose proof lem_red_beta_bot_refl_0; pose proof lem_red_beta_bot_refl; pose proof lem_red_beta_bot_trans;
+  pose proof lem_red_beta_bot_step; pose proof lem_red_beta_bot_step_rev;
+  pose proof lem_red_beta_bot_redex_beta; pose proof lem_red_beta_bot_redex_bot;
+  pose proof lem_step_beta_bot_to_red_beta_bot; pose proof lem_red_beta_to_red_beta_bot;
+  pose proof lem_step_beta_to_red_beta_bot; pose proof lem_step_beta_to_step_beta_bot;
+  pose proof lem_red_beta_bot_app; pose proof lem_red_beta_bot_abs;
+  pose proof lem_red_beta_bot_redex_U;
+  autounfold with shints in *.
+
+(******************************************************************************)
+
+Lemma lem_beta_bot_redex_shift_closed : shift_closed (beta_bot_redex U).
+Proof.
+  unfold beta_bot_redex, shift_closed.
+  pose lem_beta_redex_shift_closed; pose lem_bot_redex_shift_closed; ycrush.
+Qed.
+
+Lemma lem_step_beta_bot_shift_closed : shift_closed (step_beta_bot U).
+Proof.
+  unfold step_beta_bot.
+  pose lem_beta_bot_redex_morphism; pose lem_comp_shift_closed; pose lem_beta_bot_redex_shift_closed; scrush.
+Qed.
+
+Lemma lem_red_beta_bot_shift_closed : shift_closed (red_beta_bot U).
+Proof.
+  unfold red_beta.
+  pose lem_step_beta_bot_morphism; pose lem_star_shift_closed; pose lem_step_beta_bot_shift_closed; scrush.
+Qed.
+
+Lemma lem_inf_beta_bot_shift_closed : shift_closed (inf_beta_bot U).
+Proof.
+  pose lem_inf_shift_closed; pose lem_red_beta_bot_shift_closed; scrush.
+Qed.
+
+Lemma lem_inf_beta_bot_refl : reflexive term (inf_beta_bot U).
+Proof.
+  unfold inf_beta_bot, red_beta_bot; pose lem_inf_refl; scrush.
+Qed.
+
+Lemma lem_inf_beta_bot_prepend : forall x y z, red_beta_bot U x y -> inf_beta_bot U y z -> inf_beta_bot U x z.
+Proof.
+  unfold inf_beta_bot, red_beta_bot.
+  pose lem_step_beta_bot_morphism; pose lem_inf_prepend; eauto.
+Qed.
+
+Lemma lem_inf_beta_bot_prepend_red_beta :
+  forall x y z, red_beta x y -> inf_beta_bot U y z -> inf_beta_bot U x z.
+Proof.
+  Reconstr.reasy (lem_red_beta_to_red_beta_bot, lem_inf_beta_bot_prepend) Reconstr.Empty.
+Qed.
+
+Lemma lem_red_beta_bot_to_inf_beta_bot : forall x y, red_beta_bot U x y -> inf_beta_bot U x y.
+Proof.
+  unfold inf_beta_bot, red_beta_bot.
+  eauto using lem_star_to_inf, lem_step_beta_bot_morphism.
+Qed.
+
+Lemma lem_inf_beta_bot_app :
+  forall x x' y y', inf_beta_bot U x x' -> inf_beta_bot U y y' -> inf_beta_bot U (app x y) (app x' y').
+Proof.
+  pose_red_beta_bot; pose lem_inf_beta_bot_refl; coinduction.
+Qed.
+
+Lemma lem_inf_beta_bot_abs : forall x x', inf_beta_bot U x x' -> inf_beta_bot U (abs x) (abs x').
+Proof.
+  pose_red_beta_bot; pose lem_inf_beta_bot_refl; coinduction.
+Qed.
+
+Lemma lem_inf_beta_to_inf_beta_bot : forall x y, inf_beta x y -> inf_beta_bot U x y.
+Proof.
+  unfold inf_beta, inf_beta_bot, red_beta, red_beta_bot.
+  pose lem_step_beta_to_step_beta_bot; pose lem_inf_subset; ycrush.
+Qed.
+
+Ltac pose_inf_beta_bot := pose proof lem_inf_beta_bot_refl; pose proof lem_inf_beta_to_inf_beta_bot;
+                          pose proof lem_red_beta_bot_to_inf_beta_bot; pose proof lem_inf_beta_bot_prepend;
+                          pose proof lem_inf_beta_bot_prepend_red_beta;
+                          pose proof lem_inf_beta_bot_app; pose proof lem_inf_beta_bot_abs;
+                          autounfold with shints in *.
+
+(************************************************************************************************)
+
+Lemma lem_par_bot_to_inf_beta_bot : forall t s, par_bot U t s -> inf_beta_bot U t s.
+Proof.
+  pose_red_beta_bot; pose_inf_beta_bot; coinduction.
+Qed.
+
+Lemma lem_par_bot_over_step_beta :
+  forall t1 t2 t3, par_bot U t1 t2 -> step_beta t2 t3 -> exists s, step_beta t1 s /\ par_bot U s t3.
+Proof.
+  intros t1 t2 t3 H1 H.
+  revert t1 H1.
+  induction H; intros.
+  - inversion_clear H; subst.
+    rewrite H0 in H1.
+    inversion_clear H1; subst; [ unfold bot_redex in *; ycrush | idtac ].
+    inversion_clear H; subst; [ unfold bot_redex in *; ycrush | idtac ].
+    assert (par_bot U (x1 [0 := y0]) (t0 [0 := t2])) by eauto using lem_par_bot_subst.
+    exists (x1 [0 := y0]).
+    rewrite H2.
+    pose lem_step_beta_redex; ycrush.
+  - inversion_clear H1; subst; [ unfold bot_redex in *; ycrush | idtac ].
+    generalize (IHcomp_clos x0 H2); intro; sintuition.
+    exists (app s y0).
+    rewrite <- H0.
+    pose_term_eq; yelles 1.
+  - inversion_clear H1; subst; [ unfold bot_redex in *; ycrush | idtac ].
+    generalize (IHcomp_clos y0 H3); intro; sintuition.
+    exists (app x0 s).
+    rewrite <- H0.
+    pose_term_eq; yelles 1.
+  - inversion_clear H1; subst; [ unfold bot_redex in *; ycrush | idtac ].
+    generalize (IHcomp_clos x0 H0); intro; sintuition.
+    pose_term_eq; yelles 1.
+Qed.
+
+Lemma lem_par_bot_over_red_beta :
+  forall t1 t2 t3, par_bot U t1 t2 -> red_beta t2 t3 -> exists s, red_beta t1 s /\ par_bot U s t3.
+Proof.
+  intros t1 t2 t3 H1 H.
+  revert t1 H1.
+  destruct H as [n H].
+  induction H; pose lem_par_bot_trans; pose lem_par_bot_over_step_beta; pose_red_beta; ycrush.
+Qed.
+
+Lemma lem_step_beta_bot_disj : forall t s, step_beta_bot U t s -> step_beta t s \/ step_bot U t s.
+Proof.
+  induction 1.
+  - unfold beta_bot_redex in *; ycrush.
+  - sintuition; [ left | right ]; csolve.
+  - sintuition; [ left | right ]; csolve.
+  - sintuition; [ left | right ]; csolve.
+Qed.
+
+Lemma lem_red_beta_bot_decompose : forall t s, red_beta_bot U t s -> exists r, red_beta t r /\ par_bot U r s.
+Proof.
+  intros t s H.
+  destruct H as [n H].
+  induction H.
+  - pose lem_par_bot_refl; pose_red_beta; ycrush.
+  - assert (HH: step_beta x y \/ step_bot U x y) by eauto using lem_step_beta_bot_disj.
+    destruct HH;
+      pose lem_step_bot_to_par_bot; pose lem_par_bot_trans; pose lem_par_bot_over_red_beta;
+        pose_red_beta; ycrush.
+Qed.
+
+Corollary cor_par_bot_over_red_beta_bot :
+  forall t1 t2 t3, par_bot U t1 t2 -> red_beta_bot U t2 t3 ->
+                   exists s, red_beta t1 s /\ par_bot U s t3.
+Proof.
+  intros t1 t2 t3 H1 H2.
+  generalize (lem_red_beta_bot_decompose t2 t3 H2).
+  intro H.
+  destruct H as [r H].
+  destruct H as [H3 H4].
+  generalize (lem_par_bot_over_red_beta t1 t2 r H1 H3).
+  pose lem_par_bot_over_red_beta; pose lem_par_bot_trans; ycrush.
+Qed.
+
+Lemma lem_inf_beta_bot_prepend_par_bot :
+  forall t1 t2 t3, par_bot U t1 t2 -> inf_beta_bot U t2 t3 -> inf_beta_bot U t1 t3.
+Proof.
+  coinduct CH on 4.
+  - clear CH.
+    Reconstr.rcrush (lem_par_bot_to_inf_beta_bot, lem_inf_beta_bot_prepend,
+                     lem_red_beta_to_red_beta_bot, cor_par_bot_over_red_beta_bot)
+                    Reconstr.Empty.
+  - clear CH.
+    Reconstr.rcrush (lem_par_bot_to_inf_beta_bot, cor_par_bot_over_red_beta_bot,
+                     lem_inf_beta_bot_prepend_red_beta) Reconstr.Empty.
+  - generalize (cor_par_bot_over_red_beta_bot t1 t2 (app x y) H H1).
+    intro; simp_hyps.
+    inversion H5; subst.
+    + clear CH; pose_red_beta_bot; ycrush.
+    + apply inf_clos_app with (x := x0) (y := y0).
+      * clear CH; pose lem_red_beta_to_red_beta_bot; ycrush.
+      * eapply CH; clear CH; eauto.
+      * eapply CH; clear CH; eauto.
+  - generalize (cor_par_bot_over_red_beta_bot t1 t2 (abs x) H H1).
+    intro; simp_hyps.
+    inversion H4; subst.
+    + clear CH; pose_red_beta_bot; ycrush.
+    + apply inf_clos_abs with (x := x0).
+      * clear CH; pose lem_red_beta_to_red_beta_bot; ycrush.
+      * eapply CH; clear CH; eauto.
+Qed.
+
+(************************************************************************************************)
+
+Lemma lem_par_bot_app_choice :
+  forall t s1 s2, par_bot U t (app s1 s2) -> { p : term * term | t = app (fst p) (snd p) /\
+                                                                 par_bot U (fst p) s1 /\ par_bot U (snd p) s2 }.
+Proof.
+  intros.
+  apply constructive_indefinite_description.
+  generalize (lem_par_bot_app t s1 s2 H); intro; sintuition.
+  exists (t1, t2).
+  ycrush.
+Qed.
+
+Lemma lem_par_bot_abs_choice :
+  forall t y, par_bot U t (abs y) -> { x | t = abs x /\ par_bot U x y }.
+Proof.
+  intros.
+  apply constructive_indefinite_description.
+  apply lem_par_bot_abs.
+  assumption.
+Qed.
+
+Lemma lem_red_beta_bot_decompose_choice :
+  forall t s, red_beta_bot U t s -> { r | red_beta t r /\ par_bot U r s }.
+Proof.
+  intros.
+  apply constructive_indefinite_description.
+  apply lem_red_beta_bot_decompose.
+  assumption.
+Qed.
+
+(************************************************************************************************)
+
+CoFixpoint F_inf_beta_bot_decompose (t s : term) (p : inf_beta_bot U t s) : term.
+destruct (lem_inf_clos_cases t s p).
+- destruct (lem_red_beta_bot_decompose_choice t bot r).
+  exact x.
+- destruct (lem_red_beta_bot_decompose_choice t (var n) r).
+  exact x.
+- destruct (lem_red_beta_bot_decompose_choice t (app x y) r).
+  destruct a.
+  destruct (lem_par_bot_app_choice x0 x y H0).
+  destruct a.
+  assert (HH1: inf_beta_bot U (fst x1) x') by (pose lem_inf_beta_bot_prepend_par_bot; ycrush).
+  assert (HH2: inf_beta_bot U (snd x1) y') by (pose lem_inf_beta_bot_prepend_par_bot; ycrush).
+  exact (app (F_inf_beta_bot_decompose (fst x1) x' HH1) (F_inf_beta_bot_decompose (snd x1) y' HH2)).
+- destruct (lem_red_beta_bot_decompose_choice t (abs x) r).
+  destruct a.
+  destruct (lem_par_bot_abs_choice x0 x H0).
+  destruct a.
+  assert (HH: inf_beta_bot U x1 x') by (pose lem_inf_beta_bot_prepend_par_bot; ycrush).
+  exact (abs (F_inf_beta_bot_decompose x1 x' HH)).
+Defined.
+
+Theorem thm_inf_beta_bot_decompose :
+  forall t s, inf_beta_bot U t s -> exists r, inf_beta t r /\ par_bot U r s.
+Proof.
+  enough (exists f, forall t s (p : inf_beta_bot U t s),
+               inf_beta t (f t s p) /\ par_bot U (f t s p) s) by ycrush.
+  exists F_inf_beta_bot_decompose.
+  split.
+  - revert t s p.
+    cofix CH.
+    intros t s p.
+    peek (F_inf_beta_bot_decompose t s p).
+    destruct (lem_inf_clos_cases t s p).
+    + clear CH; destruct (lem_red_beta_bot_decompose_choice t _ r); pose_inf_beta; ycrush.
+    + clear CH; destruct (lem_red_beta_bot_decompose_choice t _ r); pose_inf_beta; ycrush.
+    + destruct (lem_red_beta_bot_decompose_choice t (app x y) r).
+      destruct a; simpl.
+      destruct (lem_par_bot_app_choice x0 x y p0).
+      destruct a; simpl.
+      apply inf_clos_app with (x := fst x1) (y := snd x1).
+      * clear CH; pose_red_beta_bot; ycrush.
+      * eapply CH; clear CH; eauto.
+      * eapply CH; clear CH; eauto.
+    + destruct (lem_red_beta_bot_decompose_choice t (abs x) r).
+      destruct a; simpl.
+      destruct (lem_par_bot_abs_choice x0 x p0).
+      destruct a; simpl.
+      apply inf_clos_abs with (x := x1).
+      * clear CH; pose_red_beta_bot; ycrush.
+      * eapply CH; clear CH; eauto.
+  - revert t s p.
+    cofix CH.
+    intros t s p.
+    peek (F_inf_beta_bot_decompose t s p).
+    destruct (lem_inf_clos_cases t s p).
+    + clear CH; destruct (lem_red_beta_bot_decompose_choice t _ r); ycrush.
+    + clear CH; destruct (lem_red_beta_bot_decompose_choice t _ r); ycrush.
+    + destruct (lem_red_beta_bot_decompose_choice t (app x y) r).
+      destruct a; simpl.
+      destruct (lem_par_bot_app_choice x0 x y p0).
+      destruct a; simpl.
+      apply par_clos_app.
+      * eapply CH.
+      * eapply CH.
+    + destruct (lem_red_beta_bot_decompose_choice t (abs x) r).
+      destruct a; simpl.
+      destruct (lem_par_bot_abs_choice x0 x p0).
+      destruct a; simpl.
+      apply par_clos_abs.
+      eapply CH.
 Qed.
 
 End Botred.
+
+(************************************************************************************************)
+
+Section Botred_strong.
+
+Variable U : term -> Prop.
+Variable Hs : strongly_meaningless U.
+
+Corollary cor_inf_beta_bot_preserves_U_rev : forall t s, U s -> inf_beta_bot U t s -> U t.
+Proof.
+  destruct Hs as [Hm He].
+  intros t s Hu H.
+  generalize (thm_inf_beta_bot_decompose U Hm t s H).
+  intros; sintuition.
+  assert (U r) by (apply lem_par_bot_preserves_U_rev with (t := s); assumption).
+  ycrush.
+Qed.
+
+Lemma lem_inf_beta_bot_to_bot_redex :
+  forall t s u, inf_beta_bot U t s -> bot_redex U s u -> inf_beta_bot U t u.
+Proof.
+  destruct Hs as [Hm He].
+  unfold bot_redex.
+  intros.
+  assert (U t) by (pose cor_inf_beta_bot_preserves_U_rev; ycrush).
+  apply lem_red_beta_bot_to_inf_beta_bot; auto.
+  pose lem_red_beta_bot_redex_U; ycrush.
+Qed.
+
+Lemma lem_inf_beta_bot_append_par_bot :
+  forall t t' s, inf_beta_bot U t t' -> par_bot U t' s -> inf_beta_bot U t s.
+Proof.
+  destruct Hs as [Hm He].
+  coinduct CH.
+  - clear CH; destruct s; sauto.
+  - clear CH; destruct s.
+    + intro H1; inversion H1; subst; eapply lem_inf_beta_bot_to_bot_redex; eauto.
+    + intro H1; inversion H1; subst; [ unfold bot_redex in *; ycrush | assumption ].
+    + sauto.
+    + sauto.
+  - csolve CH using eauto.
+    clear CH; eapply lem_inf_beta_bot_to_bot_redex; eauto.
+  - csolve CH using eauto.
+    clear CH; eapply lem_inf_beta_bot_to_bot_redex; eauto.
+Qed.
+
+Corollary cor_inf_beta_bot_append_red_beta :
+  forall t s r, inf_beta_bot U t s -> red_beta s r -> inf_beta_bot U t r.
+Proof.
+  destruct Hs as [Hm He].
+  intros t s r H1 H2.
+  generalize (thm_inf_beta_bot_decompose U Hm t s H1); intro HH.
+  destruct HH as [ t' [ H3 H4 ]].
+  generalize (lem_par_bot_over_red_beta U Hm t' s r H4 H2); intro HH.
+  destruct HH as [ s' [ H5 H6 ]].
+  assert (inf_beta_bot U t s') by (apply lem_inf_beta_to_inf_beta_bot; pose_inf_beta; ycrush).
+  eapply lem_inf_beta_bot_append_par_bot; eauto.
+Qed.
+
+End Botred_strong.
+
+Ltac pose_red_beta_bot :=
+  pose proof lem_red_beta_bot_refl_0; pose proof lem_red_beta_bot_refl; pose proof lem_red_beta_bot_trans;
+  pose proof lem_red_beta_bot_step; pose proof lem_red_beta_bot_step_rev;
+  pose proof lem_red_beta_bot_redex_beta; pose proof lem_red_beta_bot_redex_bot;
+  pose proof lem_step_beta_bot_to_red_beta_bot; pose proof lem_red_beta_to_red_beta_bot;
+  pose proof lem_step_beta_to_red_beta_bot; pose proof lem_step_beta_to_step_beta_bot;
+  pose proof lem_red_beta_bot_app; pose proof lem_red_beta_bot_abs;
+  pose proof lem_red_beta_bot_redex_U;
+  autounfold with shints in *.
+
+Ltac pose_inf_beta_bot := pose proof lem_inf_beta_bot_refl; pose proof lem_inf_beta_to_inf_beta_bot;
+                          pose proof lem_red_beta_bot_to_inf_beta_bot; pose proof lem_inf_beta_bot_prepend;
+                          pose proof lem_inf_beta_bot_prepend_red_beta;
+                          pose proof lem_inf_beta_bot_app; pose proof lem_inf_beta_bot_abs;
+                          autounfold with shints in *.
