cases.v
@@ -1,0 +1,21 @@
+
+Require Export Logic.IndefiniteDescription.
+
+Require Import defs.
+Require Import tactics.
+
+Inductive inf_clos_cases (R : relation term) : term -> term -> Set :=
+| inf_clos_cases_bot : forall t : term, R t bot -> inf_clos_cases R t bot
+| inf_clos_cases_var : forall (t : term) (n : nat), R t (var n) -> inf_clos_cases R t (var n)
+| inf_clos_cases_app : forall t x y x' y' : term,
+    R t (app x y) -> inf_clos R x x' -> inf_clos R y y' -> inf_clos_cases R t (app x' y')
+| inf_clos_cases_abs : forall t x x' : term, R t (abs x) -> inf_clos R x x' -> inf_clos_cases R t (abs x').
+
+Lemma lem_inf_clos_cases {R : relation term} : forall t s, inf_clos R t s -> inf_clos_cases R t s.
+Proof.
+  enough (H: forall t s, inf_clos R t s -> { p : inf_clos_cases R t s | True }) by
+      (intros t s H0; generalize (H t s H0); ycrush).
+  enough (forall t s, inf_clos R t s -> exists p : inf_clos_cases R t s, True) by
+      (intros; apply constructive_indefinite_description; ycrush).
+  yelles 2.
+Qed.
