Makefile
@@ -1,4 +1,4 @@
-all : tactics.vo star.vo defs.vo equality.vo basics.vo beta.vo botred.vo
+all : tactics.vo star.vo defs.vo equality.vo basics.vo beta.vo botred.vo cases.vo
 
 tactics.vo : tactics.v
 	coqc tactics.v
@@ -6,21 +6,23 @@ tactics.vo : tactics.v
 defs.vo : defs.v
 	coqc defs.v
 
+cases.vo : cases.v defs.vo
+	coqc cases.v
+
 equality.vo : equality.v defs.vo tactics.vo
 	coqc equality.v
 
 star.vo : star.v defs.vo tactics.vo equality.vo
 	coqc star.v
 
-basics.vo : basics.v equality.vo defs.vo tactics.vo equality.vo
+basics.vo : basics.v equality.vo defs.vo tactics.vo star.vo equality.vo
 	coqc basics.v
 
 beta.vo : beta.v basics.vo
 	coqc beta.v
 
-botred.vo : botred.v beta.vo
+botred.vo : botred.v beta.vo cases.vo
 	coqc botred.v
 
 clean:
 	rm -f .*.aux *.vo *.glob
-
